\section{Step 2: Translations}

The a (very informal) definition of \simple\embed is as follows:

\begin{itemize}
\item $\simple{H}$: Create assembler code to malloc and initialize the heap
  values.
\item $\simple{R}$: Append assembler code to setup the registers.
\item $\simple{I}$: Convert $\simple{I}$ to assembler and append it.
\item $\simple{G}$: Convert each each global into assembler-code and append them.
\item Finally run an assembler over the generated text to create machine code.
\end{itemize}

Defining \simple\embedp is somewhat more complicated, and is outside the scope
of this thesis. Finally \high\embed is this function:

{\footnotesize
\[\begin{array}{l}
\begin{array}{ll}
\rlap{$\drop{w} : \high w -> \simple{w}$} \\
\drop{w}(\mathtt{globval}\ \ell_g) &= \mathtt{globval}\ \ell_g \\
\drop{w}(\mathtt{heapval}\ \ell_h) &= \mathtt{heapval}\ \ell_h \\
\drop{w}(\mathtt{int}\ i) &= \mathtt{int}\ i \\
\drop{w}(\mathtt{ns}) &= \mathtt{ns} \\
\drop{w}(\mathtt{uninit}\ \tau) &= \mathtt{uninit} \\
\drop{w}(\Lambda\ \Delta.w[\theta_1, \dots, \theta_n]) &= \drop{w}(w) \\\\

\rlap{$\drop{v} : \high v -> \simple{v}$} \\
\drop{v}(\mathtt{globval}\ \ell_g) &= \mathtt{globval}\ \ell_g \\
\drop{v}(\mathtt{reg}\ r) &= \mathtt{reg}\ r \\
\drop{v}(\mathtt{int}\ i) &= \mathtt{int}\ i \\
\drop{v}(\mathtt{uninit}\ \tau) &= \mathtt{uninit} \\
\drop{v}(\Lambda\ \Delta \cdot v[\theta_1, \dots, \theta_n]) &= \drop{v}(v)
\end{array} \\\\

\begin{array}{l}
\drop{g} : \high g -> \simple{g} \\
\drop{g}(\mathtt{code}\ \forall[\Delta]\Gamma.I) = \mathtt{code}\ (\drop{I}(I)) \\\\

\drop{G} : \high G -> \simple{G} \\
\drop{G}(\{\ell_{g,1} |-> g_1, \dots, \ell_{g,n} |-> g_n\}) = \{\ell_{g,1} |-> \drop{g}(g_1), \dots, \ell_{g,n} |-> \drop{g}(g_n)\} \\\\

\drop{h} : \high h -> \simple{h} \\
\drop{h}(\langle w_1, \dots, w_n \rangle) = \langle \drop{w}(w_1), \dots \drop{w}(w_n)\rangle \\\\

\drop{H} : \high H -> \simple{H} \\
\drop{H}(\{\ell_{h,1} |-> h_1, \dots, \ell_{h,n} |-> h_n\}) = \{\ell_{h,1} |-> \drop{h}(h_1), \dots, \ell_{h,n} |-> \drop{h}(h_n)\}
\end{array} \\\\

\begin{array}{ll}
\rlap{$\drop{S} : \high S -> \simple{S}$} \\
\drop{S}(\mathtt{nil}) &= \mathtt{nil} \\
\drop{S}(w :: S) &= \drop{w}(w) :: \drop{S}(S) \\
\end{array} \\\\

\begin{array}{l}
\drop{R} : \high R -> \simple{R} \\
\drop{R}(\{\mathtt{sp} |-> S, \mathtt{r}_1 |-> w_1, \dots, \mathtt{r}_{r_{max}} |-> w_{r_{max}}\})\\
\quad\quad\quad\quad = \{\mathtt{sp} |-> \drop{S}(S), \mathtt{r}_1 |-> \drop{w}(w_1), \dots, \mathtt{r}_{r_{max}} |-> \drop{w}(w_{r_{max}})\}
\end{array} \\\\

\begin{array}{ll}
\rlap{$\drop{\iota} : \high\iota -> \simple\iota$} \\
\drop{\iota}(\mathtt{add}\ r, r, v) &= \mathtt{add}\ r, r, \drop{v}(v) \\
\drop{\iota}(\mathtt{sub}\ r, r, v) &= \mathtt{sub}\ r, r, \drop{v}(v) \\
\drop{\iota}(\mathtt{salloc}\ n) &= \mathtt{salloc}\ n \\
\drop{\iota}(\mathtt{sfree}\ n) &= \mathtt{sfree}\ n \\
\drop{\iota}(\mathtt{ld}\ r, \mathtt{sp}(n)) &= \mathtt{ld}\ r, \mathtt{sp}(n) \\
\drop{\iota}(\mathtt{st}\ \mathtt{sp}(n), r) &= \mathtt{st}\ \mathtt{sp}(n), r \\
\drop{\iota}(\mathtt{ld}\ r, r(n)) &= \mathtt{ld}\ r, r(n) \\
\drop{\iota}(\mathtt{st}\ r(n), r) &= \mathtt{st}\ r(n), r \\
\drop{\iota}(\mathtt{malloc}\ r, \langle \tau_1, \dots, \tau_n \rangle) &= \mathtt{malloc}\ r, n \\
\drop{\iota}(\mathtt{mov}\ r, v) &= \mathtt{mov}\ r, \drop{v}(v) \\
\drop{\iota}(\mathtt{beq}\ r, v) &= \mathtt{beq}\ r, \drop{v}(v) \\
\drop{\iota}(\mathtt{halt}) &= \mathtt{halt} \\
\end{array} \\\\

\begin{array}{ll}
\drop{I} : \high I -> \simple{I} \\
\drop{I}(\iota ; I) &= \drop{\iota}(\iota) ; \drop{I}(I) \\
\drop{I}(\mathtt{jmp}\ v) &= \mathtt{jmp}\ (\drop{v}(v))
\end{array} \\\\

\begin{array}{l}
\drop{C} : \high C -> \simple{C} \\
\drop{C}(H, R, I) = (\drop{H}(H), \drop{R}(R), \drop{I}(I)) \\\\

\drop{P} : \high P -> \simple{P} \\
\drop{P}(G, H, R, I) = (\drop{G}(G), \drop{H}(H), \drop{R}(R), \drop{I}(I)) \\\\

\high\embed : \high P -> \simple{P} \\
\high\embed(P) = \drop{P}(P) \\
\high\embed(\high\halt) = \simple\halt \\
\end{array} \\\\

\end{array}\]
}
