\subsection{Semantics}

We are now able to implement the semantics for our language: \\

\fbox{$\evalregs{R^\circ}{v^\circ}{w^\circ}$}
\begin{mathpar}
\infer{ }{
  \evalregs{R^\circ}{\mathtt{globval}\ \ell_g}{\mathtt{globval}\ \ell_g}
} \and
\infer{
  (r \mapsto w^\circ) \in R^\circ
}{
  \evalregs{R^\circ}{\mathtt{reg}\ r}{w^\circ}
} \and
\infer{ }{
  \evalregs{R^\circ}{\mathtt{int}\ i}{\mathtt{int}\ i}
} \and
\infer{ }{
  \evalregs{R^\circ}{\mathtt{ns}}{\mathtt{ns}}
} \and
\infer{ }{
  \evalregs{R^\circ}{\mathtt{uninit}}{\mathtt{uninit}}
}
\end{mathpar}

\fbox{$\execis{G^\circ}{H^\circ, R^\circ, I^\circ}{H^\circ{}', R^\circ{}', I^\circ{}'}$}
\begin{mathpar}
\infer{
  \evalregs{R^\circ}{v^\circ}{\mathtt{int}\ i_1} \and
  (\mathtt{r}_s \mapsto \mathtt{int}\ i_2) \in R^\circ
}{
  \execis{G^\circ}
    {H^\circ, R^\circ, (\mathtt{add}\ r_d, r_s, v^\circ) ; I^\circ}
    {H^\circ, R^\circ\{r_d \mapsto \mathtt{int}\ (i_1 + i_2)\}, I^\circ}
} \and
\infer{
  \evalregs{R^\circ}{v^\circ}{\mathtt{int}\ i_1} \and
  (r_s \mapsto \mathtt{int}\ i_2) \in R^\circ
}{
  \execis{G^\circ}
    {H^\circ, R^\circ, (\mathtt{sub}\ r_d, r_s, v^\circ) ; I^\circ}
    {H^\circ, R^\circ\{r_d |-> \mathtt{int}\ (i_1 - i_2)\}, I^\circ}
} \and
\infer{
  (\mathtt{sp} |-> S^\circ) \in R^\circ \and
  S^\circ{}' = \overbrace{\mathtt{ns} :: \dots :: \mathtt{ns}}^n :: S^\circ
}{
  \execis{G^\circ}
    {H^\circ, R^\circ, \mathtt{salloc}\ n ; I^\circ}
    {H^\circ, R^\circ\{\mathtt{sp} |-> S^\circ{}'\}, I^\circ}
} \and
\infer{
  (\mathtt{sp} |-> S^\circ) \in R^\circ \and
  S^\circ = \overbrace{w^\circ_1 :: \dots :: w^\circ_n}^n :: S^\circ{}'
}{
  \execis{G^\circ}
    {H^\circ, R^\circ, \mathtt{sfree}\ n ; I^\circ}
    {H^\circ, R^\circ\{\mathtt{sp} |-> S^\circ{}'\}, I^\circ}
} \and
\infer{
  (\mathtt{sp} |-> S^\circ) \in R^\circ \and
  \lookup{S^\circ}{n}{w^\circ}
}{
  \execis{G^\circ}
    {H^\circ, R^\circ, (\mathtt{ld}\ r_d, \mathtt{sp}(n)) ; I^\circ}
    {H^\circ, R^\circ\{r_d |-> w^\circ\}, I^\circ}
} \and
\infer{
  (r_s |-> \mathtt{heapval}\ \ell_h) \in R^\circ \and
  (\ell_h |-> h^\circ) \in H \and
  \lookup{h^\circ}{n}{w^\circ}
}{
  \execis{G^\circ}
    {H^\circ, R^\circ, (\mathtt{ld}\ r_d, r_s(n)) ; I^\circ}
    {H^\circ, R^\circ\{r_d |-> w^\circ\}, I^\circ}
} \and
\infer{
  (r_s |-> w^\circ) \in R^\circ \and
  (\mathtt{sp} |-> S^\circ) \in R^\circ \and
  \update{S^\circ}{n}{w^\circ}{S^\circ{}'}
}{
  \execis{G^\circ}
    {H^\circ, R^\circ, (\mathtt{st}\ \mathtt{sp}(n), r_s) ; I^\circ}
    {H^\circ, R^\circ\{\mathtt{sp} |-> S^\circ{}'\}, I^\circ}
} \and
\infer{
  (r_s |-> w^\circ) \in R^\circ \and
  (r_d |-> \mathtt{heapval}\ \ell_h) \in R^\circ \and
  (\ell_h |-> h^\circ) \in H^\circ \and
  \update{h^\circ}{n}{w^\circ}{h^\circ{}'}
}{
  \execis{G^\circ}
    {H^\circ, R^\circ, (\mathtt{st}\ r_d(n), r^\circ) ; I^\circ}
    {H^\circ\{\ell_h |-> h^\circ{}'\}, R^\circ, I^\circ}
} \and
\infer{
  \ell_h \not\in \mathbf{Keys}(H) \and
  h^\circ = \overbrace{\langle \mathtt{uninit}, \dots, \mathtt{uninit} \rangle}^n
}{
  \execis{G^\circ}
    {H^\circ, R^\circ, (\mathtt{malloc}\ r_d, n) ; I^\circ}
    {H^\circ \cup \{\ell_h |-> h^\circ\}, R\{r_d |-> \mathtt{heapval}\ \ell_h\}, I^\circ}
} \and
\infer{
  \evalregs{R^\circ}{v^\circ}{w^\circ}
}{
  \execis{G^\circ}
    {H^\circ, R^\circ, (\mathtt{mov}\ r_d, v^\circ) ; I^\circ}
    {H^\circ, R^\circ\{r_d |-> w^\circ\}, I^\circ}
} \and
\infer{
  (r |-> \mathtt{int}\ 0) \in R^\circ \and
  \evalregs{R^\circ}{v^\circ}{\mathtt{globval}\ \ell_g} \and
  \lookup{G^\circ}{\ell_g}{\mathtt{code}\ I^\circ{}'}
}{
  \execis{G^\circ}
    {H^\circ, R^\circ, (\mathtt{beq}\ r, v^\circ) ; I^\circ}
    {H^\circ, R^\circ, I^\circ{}'}
} \and
\infer{
  (r |-> \mathtt{int}\ i) \in R^\circ \and
  i \neq 0
}{
  \execis{G^\circ}
    {H^\circ, R^\circ, (\mathtt{beq}\ r, v^\circ) ; I^\circ}
    {H^\circ, R^\circ, I^\circ}
} \and
\infer{
  \evalregs{R^\circ}{v^\circ}{\mathtt{globval}\ \ell_g} \and
  \lookup{G^\circ}{\ell_g}{\mathtt{code}\ I^\circ{}'}
}{
  \execis{G^\circ}
    {H^\circ, R^\circ, \mathtt{jmp}\ v^\circ}
    {H^\circ, R^\circ, I^\circ{}'}
}
\end{mathpar}

\fbox{$P^\circ -> P^\circ{}'$}
\begin{mathpar}
\infer{
  \execis{G^\circ}{H^\circ, R^\circ, I^\circ}{H^\circ{}', R^\circ{}', I^\circ{}'}
}{
  (G^\circ, H^\circ, R^\circ, I^\circ) -> (G^\circ, H^\circ{}', R^\circ{}', I^\circ{}')
}
\end{mathpar}

\fbox{$\done{P^\circ}$}
\begin{mathpar}
\infer{ }{
  \done{(G^\circ, H^\circ, R^\circ, \mathtt{halt})}
}
\end{mathpar}

\begin{lemma}[Determinism]
  \label{thm:determinism}
  Assume $P^\circ, P^\circ_1, P^\circ_2$ are programs in the simplified language. Assume
  $P^\circ -> P^\circ_1$ and $P^\circ -> P^\circ_2$. We can conclude that $P^\circ_1 = P^\circ_2$.
\end{lemma}
\begin{proof}
  By induction over the structure of $P^\circ -> P^\circ_1$.
\end{proof}
